Added new target for UTP theories and finished up basic UTP definedness theory, for now.

theories/theories/utp_definedness.thy
@@ -1,12 +1,12 @@
 (******************************************************************************)
 (* Project: Unifying Theories of Programming in HOL                           *)
-(* File: utp_defined.thy                                                      *)
+(* File: utp_definedness.thy                                                  *)
 (* Author: Victor Bandur and Simon Foster, University of York (UK)            *)
 (******************************************************************************)
 
 header {* A theory of definedness in the UTP *}
 
-theory utp_defined
+theory utp_definedness
 imports 
   "../core/utp_pred"
   "../parser/utp_pred_parser"
@@ -21,18 +21,30 @@ default_sort BOOL_SORT
 
 abbreviation "def  \<equiv> MkPlain ''def'' BoolType True"
 
-(* Add a blackboard three *)
 definition TVL :: "('a WF_PREDICATE * 'a WF_PREDICATE) \<Rightarrow> 'a WF_PREDICATE" where
-(* "TVL \<equiv> \<lambda> (P,Q). `($def \<Rightarrow> P) \<and> (Q \<Leftrightarrow> $def)`" *)
-"TVL = (\<lambda> (P,Q). `P \<lhd> $def \<rhd> \<not> Q`)"
+"TVL \<equiv> \<lambda> (P,Q). `($def \<Rightarrow> P) \<and> (Q \<Leftrightarrow> $def)`"
+(* "TVL = (\<lambda> (P,Q). `P \<lhd> $def \<rhd> \<not> Q`)" *)
+
+definition PredicateT :: "'a WF_PREDICATE \<Rightarrow> 'a WF_PREDICATE" where
+"PredicateT P = `P[true/def]`"
+
+definition DefinedT :: "'a WF_PREDICATE \<Rightarrow> 'a WF_PREDICATE" where
+"DefinedT P = `\<not> P[false/def]`"
 
 declare TVL_def [eval]
+declare PredicateT_def [eval]
+declare DefinedT_def [eval]
 
 syntax
   "_upred_tvl"     :: "upred \<Rightarrow> upred \<Rightarrow> upred" ("\<three>'(_, _')")
+  "_upred_definedt" :: "upred \<Rightarrow> upred" ("\<D>'(_')")
+  "_upred_predicatet" :: "upred \<Rightarrow> upred" ("\<P>'(_')")
 
 translations
   "_upred_tvl p q"     == "CONST TVL (p, q)"
+  "_upred_definedt p" == "CONST DefinedT p"
+  "_upred_predicatet p" == "CONST PredicateT p"
+
 
 definition TrueT :: "'a WF_PREDICATE" where
 "TrueT = `\<three>(true, true)`"
@@ -44,19 +56,29 @@ definition BotT :: "'a WF_PREDICATE" where
 "BotT = `\<not> $def`"
 
 definition NotT :: "'a WF_PREDICATE \<Rightarrow> 'a WF_PREDICATE" where
-"NotT P = `\<three>(\<not> P[true/def], \<not> P[false/def])`"
+"NotT P = `\<three>(\<not> \<P>(P), \<D>(P))`"
 
 definition OrT :: "'a WF_PREDICATE \<Rightarrow> 'a WF_PREDICATE \<Rightarrow> 'a WF_PREDICATE" where
-"OrT P Q = `\<three>(P[true/def] \<or> Q[true/def], \<not> P[false/def] \<and> \<not> Q[false/def])`"
+"OrT P Q = `\<three>(\<P>(P) \<or> \<P>(Q), \<D>(P) \<and> \<D>(Q))`"
 
 definition AndT :: "'a WF_PREDICATE \<Rightarrow> 'a WF_PREDICATE \<Rightarrow> 'a WF_PREDICATE" where
-"AndT P Q = `\<three>(P[true/def] \<and> Q[true/def], \<not> P[false/def] \<and> \<not> Q[false/def])`"
+"AndT P Q = `\<three>(\<P>(P) \<and> \<P>(Q), \<D>(P) \<and> \<D>(Q))`"
 
-definition PredicateT :: "'a WF_PREDICATE \<Rightarrow> 'a WF_PREDICATE" where
-"PredicateT P = `P[true/def]`"
+definition AllDefinedT :: "'a VAR set \<Rightarrow> 'a WF_PREDICATE" where
+"AllDefinedT xs = mkPRED {b. \<forall>x\<in>xs. \<D> (\<langle>b\<rangle>\<^sub>b x)}"
 
-definition DefinedT :: "'a WF_PREDICATE \<Rightarrow> 'a WF_PREDICATE" where
-"DefinedT P = `\<not> P[false/def]`"
+definition ExistsT :: "'a VAR set \<Rightarrow> 'a WF_PREDICATE \<Rightarrow> 'a WF_PREDICATE" where
+"ExistsT xs p = (\<exists>p xs. AllDefinedT xs \<and>p p)"
+
+notation ExistsT ("(\<exists>t _ ./ _)" [0, 10] 10)
+
+definition ForallT :: "'a VAR set \<Rightarrow> 'a WF_PREDICATE \<Rightarrow> 'a WF_PREDICATE" where
+"ForallT xs p = (\<forall>p xs. AllDefinedT xs \<Rightarrow>p p)"
+
+notation ForallT ("(\<forall>t _ ./ _)" [0, 10] 10)
+
+definition ClosureT :: "'a WF_PREDICATE \<Rightarrow> 'a WF_PREDICATE" where
+"ClosureT p = (\<forall>t VAR. p)"
 
 declare TrueT_def  [eval]
 declare FalseT_def [eval]
@@ -64,8 +86,14 @@ declare BotT_def [eval]
 declare NotT_def [eval]
 declare OrT_def [eval]
 declare AndT_def [eval]
-declare PredicateT_def [eval]
-declare DefinedT_def [eval]
+
+text {* DH for a given TVL (P, Q) ensures that P is true only when Q is also true,
+        i.e. a true valuation must also be a defined evaluation. *}
+
+definition DH :: "'a WF_PREDICATE \<Rightarrow> 'a WF_PREDICATE" where
+"DH(P) = `P \<and> (\<D>(P) \<sqsubseteq> \<P>(P))`"
+
+declare DH_def [eval]
 
 syntax
   "_upred_truet"    :: "upred" ("true\<^sub>T")
@@ -74,8 +102,8 @@ syntax
   "_upred_nott"     :: "upred \<Rightarrow> upred" ("\<not>\<^sub>T _" [40] 40)
   "_upred_andt"     :: "upred \<Rightarrow> upred \<Rightarrow> upred" (infixr "\<and>\<^sub>T" 35)
   "_upred_ort"      :: "upred \<Rightarrow> upred \<Rightarrow> upred" (infixr "\<or>\<^sub>T" 35)
-  "_upred_definedt" :: "upred \<Rightarrow> upred" ("\<D>'(_')")
-  "_upred_predicatet" :: "upred \<Rightarrow> upred" ("\<P>'(_')")
+  "_upred_clost"    :: "upred \<Rightarrow> upred" ("[_]\<^sub>T")
+  "_upred_dh"       :: "upred \<Rightarrow> upred" ("DH'(_')")
 
 translations
   "_upred_truet"    == "CONST TrueT"
@@ -84,8 +112,8 @@ translations
   "_upred_nott p"   == "CONST NotT p"
   "_upred_andt p q" == "CONST AndT p q"
   "_upred_ort p q"  == "CONST OrT p q"
-  "_upred_definedt p" == "CONST DefinedT p"
-  "_upred_predicatet p" == "CONST PredicateT p"
+  "_upred_clost p"  == "CONST ClosureT p"
+  "_upred_dh p"     == "CONST DH p"
 
 lemma TrueT_unfold:
   "`true\<^sub>T` = `$def`"
@@ -95,12 +123,8 @@ lemma FalseT_unfold:
   "`false\<^sub>T` = `false`"
   by (utp_pred_tac)
 
-definition DH :: "'a WF_PREDICATE \<Rightarrow> 'a WF_PREDICATE" where
-"DH(P) = `P \<and> (\<D>(P) \<sqsubseteq> \<P>(P))`"
-
-declare DH_def [eval]
-
-lemma DH_idem: "DH (DH P) = DH P"
+lemma DH_idem: 
+  "DH (DH P) = DH P"
   by (utp_pred_auto_tac)
 
 lemma DH_refine: "P is DH \<Longrightarrow> `\<D>(P) \<sqsubseteq> \<P>(P)`"
@@ -109,41 +133,43 @@ lemma DH_refine: "P is DH \<Longrightarrow> `\<D>(P) \<sqsubseteq> \<P>(P)`"
 lemma DH_defined_anhil: "P is DH \<Longrightarrow> `\<D>(P) \<and> \<P>(P)` = `\<P>(P)`"
   by (utp_pred_auto_tac)
 
-lemma TVL_inject: "`\<three>(\<P>(P), \<D>(P))` = P"
-  apply (simp add:TVL_def PredicateT_def DefinedT_def)
+lemma TVL_inject: "P is DH \<Longrightarrow> `\<three>(\<P>(P), \<D>(P))` = P"
+  apply (simp add:DH_def is_healthy_def TVL_def DefinedT_def PredicateT_def)
   apply (rule BoolType_aux_var_split_eq_intro[of "def"])
-  apply (simp_all add:TrueT_def TVL_def AndT_def usubst typing defined CondR_true CondR_false DH_def is_healthy_def)
+  apply (simp_all add:typing defined usubst CondR_true CondR_false)
+  apply (utp_pred_auto_tac)
+done
+
+lemma DH_TVL: "UNREST {def} Q \<Longrightarrow> `\<three>(P, Q)` is DH"
+  apply (simp add:TVL_def DH_def is_healthy_def DefinedT_def PredicateT_def usubst typing defined)
+  apply (utp_pred_auto_tac)
+done
+
+lemma DH_BotT: "`\<bottom>\<^sub>T` is DH"
+  by (utp_pred_tac, utp_expr_tac)
+
+lemma DH_TrueT: "`true\<^sub>T` is DH"
+  by (utp_pred_tac, utp_expr_tac)
+
+lemma DH_FalseT: "`false\<^sub>T` is DH"
+  by (utp_pred_tac)
+
+lemma DH_AndT: "\<lbrakk> P is DH; Q is DH \<rbrakk> \<Longrightarrow> `P \<and>\<^sub>T Q` is DH"
+  apply (simp add: AndT_def)
+  apply (rule DH_TVL)
+  apply (simp add:DefinedT_def unrest typing defined)
 done
 
 lemma TVL_left:
-  "`\<P>(\<three>(P, Q))` = `P[true/def]`"
-  by (simp add:TVL_def PredicateT_def usubst typing defined CondR_true)
+  "`\<P>(\<three>(P, Q))` = `(P \<and> Q)[true/def]`"
+  by (simp add:TVL_def PredicateT_def usubst typing defined)
 
 lemma TVL_right:
   "`\<D>(\<three>(P, Q))` = `Q[false/def]`"
-  by (simp add:TVL_def usubst typing defined unrest closure CondR_false DefinedT_def)
-
-(*
-definition DH :: "'a WF_PREDICATE \<Rightarrow> 'a WF_PREDICATE" where
-(* "DH(P) = `\<three>(P[true/def], \<not> P[false/def])`" *)
-"DH(P) = `($def \<Leftrightarrow> \<D> P) \<and> P`"
-
-declare DH_def [eval]
-*)
-
-
-lemma TVL_DH:
-  "\<lbrakk> UNREST {def} P; UNREST {def} Q; Q \<sqsubseteq> P \<rbrakk> \<Longrightarrow> `\<three>(P, Q)` is DH"
-  apply (simp add:is_healthy_def DH_def TVL_right PredicateT_def)
-  apply (simp add:TVL_def)
-  apply (rule_tac BoolType_aux_var_split_eq_intro[of "def"])
-  apply (simp_all add:typing defined usubst CondR_true CondR_false)
-  apply (utp_pred_auto_tac)
-  apply (utp_pred_auto_tac)
-done
+  by (utp_pred_tac, utp_expr_tac)
 
 lemma DefinedT_BotT:
-  "`\<not> \<D>(\<bottom>\<^sub>T)`"
+  "[\<not> \<D>(\<bottom>\<^sub>T)]"
   by (utp_pred_tac, utp_expr_tac)
 
 lemma DefinedT_TrueT:
@@ -155,51 +181,29 @@ lemma DefinedT_FalseT:
   by (utp_pred_tac)
 
 lemma TVL_extreme_point1:
-  "`\<three>(true, false)` = `true`"
+  "`\<three>(true, false)` = `\<not> $def`"
   by (utp_pred_tac)
 
 lemma TVL_extreme_point2:
   "`\<three>(false, false)` = `\<not> $def`"
   by (utp_pred_tac)
 
-(*
-lemma TVL_trade:
-  "`\<three>(P \<and> Q, Q)` = `\<three>(P, Q)`"
-  apply (utp_pred_auto_tac)
-*)
-
 lemma AndT_left_unit:
-  "`true\<^sub>T \<and>\<^sub>T P` = `P`"
+  "P is DH \<Longrightarrow> `true\<^sub>T \<and>\<^sub>T P` = `P`"
+  apply (simp add:TVL_def AndT_def DefinedT_def TrueT_def PredicateT_def)
   apply (rule BoolType_aux_var_split_eq_intro[of "def"])
-  apply (simp_all add:TrueT_def TVL_def AndT_def usubst typing defined CondR_true CondR_false)
+  apply (simp_all add:typing defined usubst)
+  apply (metis AndP_comm DH_defined_anhil DefinedT_def PredicateT_def)
 done
 
 lemma AndT_right_unit:
-  "`P \<and>\<^sub>T true\<^sub>T` = `P`"
+  "P is DH \<Longrightarrow> `P \<and>\<^sub>T true\<^sub>T` = `P`"
+  apply (simp add:TVL_def AndT_def DefinedT_def TrueT_def PredicateT_def)
   apply (rule BoolType_aux_var_split_eq_intro[of "def"])
-  apply (simp_all add:TrueT_def TVL_def AndT_def usubst typing defined CondR_true CondR_false)
+  apply (simp_all add:typing defined usubst)
+  apply (metis AndP_comm DH_defined_anhil DefinedT_def PredicateT_def)
 done
 
-lemma "`true\<^sub>T` is DH"
-  apply (simp add:is_healthy_def DH_def TrueT_def TVL_def usubst typing defined CondR_false DefinedT_def)
-  apply (utp_pred_tac)
-done
-
-lemma "`false\<^sub>T` is DH"
-  apply (simp add:is_healthy_def DH_def FalseT_def TVL_def usubst typing defined CondR_false DefinedT_def)
-  apply (utp_pred_tac)
-done
-
-lemma OrT_left_anhil:
-  "P is DH \<Longrightarrow> `true\<^sub>T \<or>\<^sub>T P` = `true`"
-  apply (simp_all add:TrueT_def TVL_def OrT_def DefinedT_def usubst typing defined CondR_true CondR_false)
-  apply (simp add: DH_def is_healthy_def)
-  apply (simp add: OrT_def)
-  by (utp_pred_tac, utp_expr_tac, auto)
-
-lemma OrT_right_anhil:
-  "`P \<or>\<^sub>T true\<^sub>T` = `$def \<Leftrightarrow> \<D> P`"
-  by (utp_pred_tac, utp_expr_tac, auto)
 
 lemma AndT_assoc:
   "`(P \<and>\<^sub>T Q) \<and>\<^sub>T R` = `P \<and>\<^sub>T Q \<and>\<^sub>T R`"
@@ -218,7 +222,11 @@ lemma OrT_commute:
   by (utp_pred_tac, utp_expr_tac, auto)
 
 lemma NotT_double: "P is DH \<Longrightarrow> `\<not>\<^sub>T \<not>\<^sub>T P` = `P`"
-  by (utp_pred_tac, utp_expr_tac, auto)
+  apply (simp add:NotT_def TVL_def PredicateT_def DefinedT_def)
+  apply (rule BoolType_aux_var_split_eq_intro[of "def"])
+  apply (simp_all add:typing defined usubst)
+  apply (utp_pred_auto_tac)
+done
 
 lemma NotT_TrueT: "`\<not>\<^sub>T true\<^sub>T` = `false\<^sub>T`"
   by (utp_pred_tac, utp_expr_tac)
